theories/lifetime/model/borrow.v
@@ -6,7 +6,7 @@ From iris.proofmode Require Import tactics.
 Set Default Proof Using "Type".
 
 Section borrow.
-Context `{!invG Σ, !lftG Σ}.
+Context `{!invG Σ, !lftG Σ userE}.
 Implicit Types κ : lft.
 
 Lemma raw_bor_create E κ P :
