theories/typing/soundness.v
@@ -35,7 +35,7 @@ Section type_soundness.
     { split. by eapply adequate_nonracing.
       intros. by eapply (adequate_not_stuck _ (main [exit_cont]%E)). }
     apply: lrust_adequacy=>?. iIntros "_".
-    iMod lft_init as (?) "#LFT". done.
+    iMod (lft_init _ lft_userE) as (?) "#LFT"; [done|solve_ndisj|].
     iMod na_alloc as (tid) "Htl". set (Htype := TypeG _ _ _ _ _).
     wp_bind (of_val main). iApply (wp_wand with "[Htl]").
     iApply (Hmain Htype [] [] $! tid 1%Qp with "LFT [] Htl [] []").
